\begin{figure}
    \centering
    \begin{gather*}
        \id[\overline{m}] \seq  f = f
        \quad
        f = f \seq \id[\overline{n}]
        \quad
        (f \seq g) \seq h = f \seq (g \seq h)
        \\[0.5em]
        \id[\epsilon] \tensor f = f
        \quad
        f \tensor \id[\epsilon] = f
        \quad
        (f \tensor g) \tensor h = f \tensor (g \tensor h)
        \\[0.5em]
        \id[\overline{m}] \tensor \id[\overline{n}] = \id[\overline{mn}]
        \quad
        (f \tensor g) \seq (h \tensor k) = (f \seq h) \tensor (g \seq k)
        \\[0.5em]
        (f \tensor g) \seq \swap{\overline{n}}{\overline{q}} = \swap{\overline{m}}{\overline{p}} \seq (g \tensor f)
        \quad
        (\swap{\overline{m}}{\overline{n}} \tensor \id[\overline{p}]) \seq (\id[\overline{n}] \tensor \swap{\overline{m}}{\overline{p}}) = \swap{\overline{m}}{\overline{np}}
        \\[0.5em]
        \swap{\epsilon}{\overline{n}} = \id[\overline{n}]
        \quad
        \swap{m}{\epsilon} = \id[\overline{m}]
        \quad
        \swap{\overline{m}}{\overline{n}} \seq \swap{\overline{n}}{\overline{m}} = \id[\overline{mn}]
    \end{gather*}
    \caption{Summary of `structural' axioms that hold in \(\smc{\generators}\).}
    \label{fig:structural-equations}
\end{figure}